partialmap.fst should be removed ...

lib/partialmap.fst
@@ -1,3 +1,170 @@
+module Set
+open Prims.PURE
+
+(*private extensional*) type set (a:Type) = a -> Tot bool
+
+assume type Equal : #a:Type -> set a -> set a -> Type
+
+(* private *) assume EqualDef : (forall (a:Type) (s1:set a) (s2:set a). Equal s1 s2 <==> (forall x. s1 x = s2 x))
+
+(* private *) assume Extensionality : (forall (a:Type) (s1:set a) (s2:set a). Equal s1 s2 <==> s1 = s2)
+
+val empty : a:Type -> Tot (set a)
+(* private *) let empty = (fun _ -> false)
+
+val singleton : a:Type -> a -> Tot (set a)
+(* private *) let singleton x = (fun y -> y = x)
+
+val union : a:Type -> set a -> set a -> Tot (set a)
+(* private *) let union s1 s2 = (fun x -> s1 x || s2 x)
+
+val intersect : a:Type -> set a -> set a -> Tot (set a)
+(* private *) let intersect s1 s2 = (fun x -> s1 x && s2 x)
+
+val complement : a:Type -> set a -> Tot (set a)
+(* private *) let complement s = (fun x -> not (s x))
+
+val mem : a:Type -> a -> set a -> Tot bool
+(* private *) let mem x s = s x
+
+val memEmpty : a:Type -> x:a -> Lemma (requires True) (ensures (not (mem x empty))) [SMTPat (mem x empty)]
+(* private *) let memEmpty (a:Type) (x:a) = ()
+
+val memSingleton : a:Type -> x:a -> y:a -> Lemma (requires True) (ensures (mem x (singleton y) == (x = y))) [SMTPat (mem x (singleton y))]
+(* private *) let memSingleton (a:Type) (x:a) (y:a) = ()
+
+val memUnion : a:Type -> s1:set a -> s2:set a -> x:a -> Lemma (requires True) (ensures (mem x (union s1 s2) = (mem x s1 || mem x s2))) [SMTPat (mem x (union s1 s2))]
+(* private *) let memUnion (a:Type) (s1:set a) (s2:set a) (x:a) = ()
+
+val memIntersect : a:Type -> s1:set a -> s2:set a -> x:a -> Lemma (requires True) (ensures (mem x (intersect s1 s2) = (mem x s1 && mem x s2))) [SMTPat (mem x (intersect s1 s2))]
+(* private *) let memIntersect (a:Type) (s1:set a) (s2:set a) (x:a) = ()
+
+val memComplement : a:Type -> s:set a -> x:a -> Lemma (requires True) (ensures (mem x (complement s) = not (mem x s))) [SMTPat (mem x (complement s))]
+(* private *) let memComplement (a:Type) (s:set a) (x:a) = ()
+
+val extensional : a:Type -> s1:set a -> s2:set a -> Lemma (requires True) (ensures (Equal s1 s2 <==> s1 = s2)) (* error: [SMTPat (Equal a s1 s2)] *)
+(* private *) let extensional (a:Type) (s1:set a) (s2:set a) = ()
+
+val equals : a:Type -> s1:set a -> s2:set a -> Lemma (requires True) (ensures (Equal s1 s2 <==> (forall x. (* error: {:pattern (mem x s1); (mem x s2)}*) mem x s1 = mem x s2))) (* error: [SMTPat (Equal a s1 s2)] *)
+(* private *) let equals (a:Type) (s1:set a) (s2:set a) = ()
+
+let minus (a:Type) (s1:set a) (s2:set a) = intersect s1 (complement s2)
+
+opaque type Subset' (a:Type) (s1:set a) (s2:set a) = (forall (x:a).{:pattern mem x s1} mem x s1 ==> mem x s2)
+
+type Subset : #a:Type -> set a -> set a -> Type = fun (a:Type) (s1:set a) (s2:set a) -> Subset' a s1 s2
+
+module Map
+open Prims.PURE
+open Set
+
+assume type t : Type -> Type -> Type
+assume logic val sel :       key:Type -> value:Type -> t key value -> key -> Tot value
+assume logic val upd :       key:Type -> value:Type -> t key value -> key -> value -> Tot (t key value)
+assume logic val const :     key:Type -> value:Type -> v:value -> Tot (t key value)
+assume logic val concat:     key:Type -> value:Type -> t key value -> t key value -> Tot (t key value)
+assume logic val contains:   key:Type -> value:Type -> t key value -> key -> Tot bool
+assume logic val equal:      key:Type -> value:Type -> t key value -> t key value -> Tot bool
+assume logic val restrict:   key:Type -> value:Type -> set key -> t key value -> Tot (t key value)
+
+assume SelUpd1:       forall (key:Type) (value:Type) (m:t key value) (k:key) (v:value).          {:pattern sel (upd m k v) k}
+                      sel (upd m k v) k == v
+
+assume SelUpd2:       forall (key:Type) (value:Type) (m:t key value) (k1:key) (k2:key) (v:value).{:pattern sel (upd m k2 v) k1}
+                      k2=!=k1 ==> sel (upd m k2 v) k1 == sel m k1
+
+assume SelConst:      forall (key:Type) (value:Type) (v:value) (k:key).                          {:pattern sel (const v) k}
+                      sel (const v) k == v
+
+assume SelRestrict:   forall (key:Type) (value:Type) (m:t key value) (ks:set key) (k:key).       {:pattern sel (restrict ks m) k}
+                      mem k ks ==> sel (restrict ks m) k == sel m k
+
+assume SelConcat1:    forall (key:Type) (value:Type) (m1:t key value) (m2:t key value) (k:key).  {:pattern sel (concat m1 m2) k}
+                      contains m2 k ==> sel (concat m1 m2) k==sel m2 k
+
+assume SelConcat1:    forall (key:Type) (value:Type) (m1:t key value) (m2:t key value) (k:key).  {:pattern sel (concat m1 m2) k}
+                      not(contains m2 k) ==> sel (concat m1 m2) k==sel m1 k
+
+assume InDomUpd1:     forall (key:Type) (value:Type) (m:t key value) (k1:key) (k2:key) (v:value).   {:pattern contains (upd m k1 v) k2}
+                      contains (upd m k1 v) k2 == (k1=k2 || contains m k2)
+
+assume InDomUpd2:     forall (key:Type) (value:Type) (m:t key value) (k1:key) (k2:key) (v:value).{:pattern contains (upd m k2 v) k1}
+                      k2=!=k1 ==> contains (upd m k2 v) k1 == contains m k1
+
+assume InDomConstMap: forall (key:Type) (value:Type) (v:value) (k:key).                          {:pattern contains (const v) k}
+                      contains (const v) k
+
+assume InDomConcat:   forall (key:Type) (value:Type) (m1:t key value) (m2:t key value) (k:key).  {:pattern contains (concat m1 m2) k}
+                      contains (concat m1 m2) k==(contains m1 k || contains m2 k)
+
+assume InDomRestrict: forall (key:Type) (value:Type) (m:t key value) (ks:set key) (k:key).       {:pattern contains (restrict ks m) k}
+                      contains (restrict ks m) k == mem k ks
+
+assume Extensional:   forall (key:Type) (value:Type) (m1:t key value) (m2:t key value).          {:pattern (equal m1 m2)}
+                      equal m1 m2 <==> m1 == m2
+
+assume Equals:        forall (key:Type) (value:Type) (m1:t key value) (m2:t key value).          {:pattern (equal m1 m2)}
+                      equal m1 m2 <==> (forall k.{:pattern (sel m1 k); (sel m2 k)} sel m1 k == sel m2 k)
+
+let const_on (key:Type) (value:Type) (dom:set key) (v:value) = restrict dom (const v)
+
+opaque type DisjointDom (key:Type) (value:Type) (m1:t key value) (m2:t key value) =
+          (forall x.{:pattern (contains m1 x)(* ; (contains m2 x) *)} contains m1 x ==> not (contains m2 x))
+
+module Heap
+open Set
+
+type aref = 
+  | Ref : a:Type -> r:ref a -> aref
+
+type refs =
+  | AllRefs : refs
+  | SomeRefs : v:set aref -> refs
+
+let no_refs  = SomeRefs empty
+let a_ref  r = SomeRefs (singleton (Ref r))
+
+assume logic val sel :       a:Type -> heap -> ref a -> Tot a
+assume logic val upd :       a:Type -> heap -> ref a -> a -> Tot heap
+assume logic val emp :       heap
+assume logic val contains :  a:Type -> heap -> ref a -> Tot bool
+assume logic val equal:      heap -> heap -> Tot bool
+assume logic val restrict:   heap -> set aref -> Tot heap
+assume logic val concat:     heap -> heap -> Tot heap
+
+assume SelUpd1:       forall (a:Type) (h:heap) (r:ref a) (v:a).            {:pattern (sel (upd h r v) r)}       
+                      sel (upd h r v) r == v
+
+assume SelUpd2:       forall (a:Type) (b:Type) (h:heap) (k1:ref a) (k2:ref b) (v:b).{:pattern (sel (upd h k2 v) k1)}     
+                      k2=!=k1 ==> sel (upd h k2 v) k1 == sel h k1
+
+assume ContainsUpd:   forall (a:Type) (b:Type) (h:heap) (k1:ref a) (k2:ref b) (v:a).{:pattern contains (upd h k1 v) k2}
+                      contains (upd h k1 v) k2 <==> (k1==k2 \/ contains h k2)
+
+assume InDomEmp:      forall (a:Type) (k:ref a).                           {:pattern contains emp k}
+                      not(contains emp k)
+
+assume Extensional:   forall (h1:heap) (h2:heap).                          {:pattern equal h1 h2}               
+                      equal h1 h2 <==> h1 == h2
+
+assume Equals:        forall (h1:heap) (h2:heap).                          {:pattern equal h1 h2}               
+                      equal h1 h2 <==> (forall (a:Type) (k:ref a).{:pattern (sel h1 k); (sel h2 k)} sel h1 k == sel h2 k)
+
+assume RestrictSel:   forall (a:Type) (h:heap) (r:set aref) (a:ref a).     {:pattern sel (restrict h r) a}
+                      mem (Ref a) r ==> sel (restrict h r) a == sel h a
+
+assume RestrictIn:    forall (a:Type) (h:heap) (r:set aref) (a:ref a).     {:pattern contains (restrict h r) a}
+                      contains (restrict h r) a == (mem (Ref a) r && contains h a)
+
+assume SelConcat:     forall (a:Type) (h1:heap) (h2:heap) (a:ref a).       {:pattern sel (concat h1 h2) a}
+                      if b2t (contains h2 a) then sel (concat h1 h2) a==sel h2 a else sel (concat h1 h2) a == sel h1 a
+
+assume ContainsConcat:forall (a:Type) (h1:heap) (h2:heap) (a:ref a).       {:pattern contains (concat h1 h2) a}
+                      contains (concat h1 h2) a == (contains h1 a || contains h2 a)
+
+type On (r:set aref) (p:(heap -> Type)) (h:heap) = p (restrict h r)
+opaque type fresh (h:heap) (refs:set aref)       = (forall (a:Type) (a:ref a).{:pattern (contains h a)} mem (Ref a) refs ==> not(contains h a))
+
 (* A logical theory of integer-indexed arrays, from [0, n) *)
 module Array
 
